AlgebraIst/TPC1.lean
@@ -1,22 +1,22 @@
 import AlgebraIst.Structures
 
 theorem ex_2_3_a {A : Type u} {G : group A} (x y z w : A) : 
-  x * y * (G.inv z) * w = G.id → y = (G.inv x) * (G.inv w) * z := by
-  intro h -- h turns into this x * y * (G.inv z) * w = G.id
+  x * y * z⁻¹ * w = G.id → y = x⁻¹ * w⁻¹ * z := by
+  intro h -- h turns into this x * y * z⁻¹ * w = G.id
   
-  replace h := congrArg (fun a => a * G.inv w) h -- apply inverse w
+  replace h := congrArg (λ a => a * w⁻¹) h -- apply inverse w
   dsimp at h -- remove the fun stuff!
   rw [G.id_lmul, G.mul_assoc, G.inv_rmul, G.mul_assoc, G.id_rmul] at h -- turns x y z^-1 w w^-1 = id * w^-1 into x y z^-1 = w^-1                
 
-  replace h := congrArg (fun a => G.inv x * a) h -- apply inverse w
+  replace h := congrArg (λ a => x⁻¹ * a) h -- apply inverse w
   dsimp at h -- remove the fun stuff!
   rw [<-G.mul_assoc, <-G.mul_assoc, G.inv_lmul, G.id_lmul] at h 
 
-  replace h := congrArg (fun a => a * z) h -- apply inverse z
+  replace h := congrArg (λ a => a * z) h -- apply inverse z
   dsimp at h -- remove the fun stuff!
   rw [G.mul_assoc, G.inv_lmul, G.id_rmul] at h
   
-  trivial -- schiappa moment
+  trivial -- schiappa moment (ignore this teach)
 
 theorem ex_2_3_b_1 {A : Type u} {G : group A} (x y z : A) :
   x * y * z = G.id -> y * z * x = G.id := by
@@ -41,4 +41,3 @@ theorem ex_2_4_b_2 {A : Type u} {G : group A} (x y z : A)
   simp [G.mul_assoc, G.inv_rmul, G.id_lmul, G.id_rmul] at h2
   rw [<-h2] at h1
   exact h1.symm
-
